OpenVM: pretty-printing of the constraints like in the Rust code

Garden/Plonky3/MExpr.v
@@ -1,4 +1,9 @@
 Require Import Garden.Plonky3.M.
+Require Import Coq.Numbers.Cyclic.Int63.PrimInt63.
+Require Export Coq.Strings.PrimString.
+
+Export PStringNotations.
+Global Open Scope pstring_scope.
 
 Module Field.
   Record t : Set := {
@@ -10,6 +15,8 @@ Module Var.
   Record t : Set := {
     index : Z;
   }.
+
+  Definition make := Build_t.
 End Var.
 
 Module Expr.
@@ -24,6 +31,9 @@ Module Expr.
   | Neg (x : t)
   | Mul (x y : t).
 
+  Definition var (index : Z) : t :=
+    Var {| Var.index := index |}.
+
   Definition constant (value : Z) : t :=
     Constant {| Field.value := value |}.
 
@@ -32,7 +42,7 @@ Module Expr.
   Definition ONE : t := constant 1.
 
   Definition not (e : t) : t :=
-    Sub e ONE.
+    Sub ONE e.
 
   Definition assert_zero (e : t) : t :=
     e.
@@ -49,6 +59,9 @@ Module Builder.
     constraints : list Expr.t;
   }.
 
+  Definition new : t :=
+    {| constraints := [] |}.
+
   Definition assert_zero (builder : t) (e : Expr.t) : t :=
     {| constraints := Expr.assert_zero e :: builder.(constraints) |}.
 
@@ -58,3 +71,129 @@ Module Builder.
   Definition assert_bool (builder : t) (e : Expr.t) : t :=
     assert_zero builder (Expr.assert_bool e).
 End Builder.
+
+Module ToRocq.
+  Class C (T : Set) : Set := {
+    to_rocq (value : T) (indent : Z) : string;
+  }.
+
+  Fixpoint indent_aux (indent : nat) : string :=
+    match indent with
+    | O => ""
+    | S n => PrimString.cat (PrimString.make 1%int63 32%int63) (indent_aux n)
+    end.
+
+  Definition indent (indent : Z) : string :=
+    indent_aux (Z.to_nat indent).
+
+  Fixpoint cats (l : list string) : string :=
+    match l with
+    | [] => ""
+    | x :: xs => PrimString.cat x (cats xs)
+    end.
+
+  Definition endl : string :=
+    "
+".
+
+  Fixpoint pstring_of_uint (n : Decimal.uint) : PrimString.string :=
+    match n with
+    | Decimal.Nil => ""%pstring
+    | Decimal.D0 n =>
+        PrimString.cat (PrimString.make 1 48%int63) (pstring_of_uint n)
+    | Decimal.D1 n =>
+        PrimString.cat (PrimString.make 1 49%int63) (pstring_of_uint n)
+    | Decimal.D2 n =>
+        PrimString.cat (PrimString.make 1 50%int63) (pstring_of_uint n)
+    | Decimal.D3 n =>
+        PrimString.cat (PrimString.make 1 51%int63) (pstring_of_uint n)
+    | Decimal.D4 n =>
+        PrimString.cat (PrimString.make 1 52%int63) (pstring_of_uint n)
+    | Decimal.D5 n =>
+        PrimString.cat (PrimString.make 1 53%int63) (pstring_of_uint n)
+    | Decimal.D6 n =>
+        PrimString.cat (PrimString.make 1 54%int63) (pstring_of_uint n)
+    | Decimal.D7 n =>
+        PrimString.cat (PrimString.make 1 55%int63) (pstring_of_uint n)
+    | Decimal.D8 n =>
+        PrimString.cat (PrimString.make 1 56%int63) (pstring_of_uint n)
+    | Decimal.D9 n =>
+        PrimString.cat (PrimString.make 1 57%int63) (pstring_of_uint n)
+    end.
+
+  Definition of_Z (z : Z) : PrimString.string :=
+    pstring_of_uint (Nat.to_uint (Z.to_nat z)).
+End ToRocq.
+
+Fixpoint string_of_expr (expr : Expr.t) (indent : Z) : string :=
+  match expr with
+  | Expr.Var var =>
+    ToRocq.cats [ToRocq.indent indent; "Variable: "; ToRocq.of_Z var.(Var.index); ToRocq.endl]
+  | Expr.IsFirstRow =>
+    ToRocq.cats [ToRocq.indent indent; "IsFirstRow"]
+  | Expr.IsLastRow =>
+    ToRocq.cats [ToRocq.indent indent; "IsLastRow"]
+  | Expr.IsTransition =>
+    ToRocq.cats [ToRocq.indent indent; "IsTransition"]
+  | Expr.Constant value =>
+    ToRocq.cats [ToRocq.indent indent; "Constant: "; ToRocq.of_Z value.(Field.value); ToRocq.endl]
+  | Expr.Add x y =>
+    ToRocq.cats [ToRocq.indent indent; "Add:"; ToRocq.endl;
+      string_of_expr x (indent + 2);
+      string_of_expr y (indent + 2)
+    ]
+  | Expr.Sub x y =>
+    ToRocq.cats [ToRocq.indent indent; "Sub:"; ToRocq.endl;
+      string_of_expr x (indent + 2);
+      string_of_expr y (indent + 2)
+    ]
+  | Expr.Neg x =>
+    ToRocq.cats [ToRocq.indent indent; "Neg:"; ToRocq.endl;
+      string_of_expr x (indent + 2)
+    ]
+  | Expr.Mul x y =>
+    ToRocq.cats [ToRocq.indent indent; "Mul:"; ToRocq.endl;
+      string_of_expr x (indent + 2);
+      string_of_expr y (indent + 2)
+    ]
+  end.
+
+Global Instance ExprIsToRocq : ToRocq.C Expr.t := {
+  to_rocq := string_of_expr;
+}.
+
+Global Instance OptionIsToRocq {T : Set} {C : ToRocq.C T} : ToRocq.C (option T) := {
+  to_rocq self indent :=
+    match self with
+    | Some x =>
+      ToRocq.cats [ToRocq.indent indent; "Some:"; ToRocq.endl;
+        ToRocq.to_rocq x (indent + 2)
+      ]
+    | None => ToRocq.cats [ToRocq.indent indent; "None"]
+    end;
+}.
+
+Global Instance ListIsToRocq {T : Set} {C : ToRocq.C T} : ToRocq.C (list T) := {
+  to_rocq self indent :=
+    ToRocq.cats (
+      [ToRocq.indent indent; "Array:"; ToRocq.endl] ++
+      List.map (fun item => ToRocq.to_rocq item (indent + 2)) self
+    );
+}.
+
+Global Instance ArrayIsToRocq {T : Set} {C : ToRocq.C T} {N : Z} : ToRocq.C (Array.t T N) := {
+  to_rocq self indent :=
+    ToRocq.to_rocq (Array.to_list self) indent
+}.
+
+Global Instance BuilderIsToRocq : ToRocq.C Builder.t := {
+  to_rocq builder indent :=
+    ToRocq.cats (
+      [ToRocq.indent indent; "Builder:"; ToRocq.endl] ++
+      List.map (fun item =>
+        ToRocq.cats [ToRocq.indent (indent + 2); "AssertZero:"; ToRocq.endl;
+          ToRocq.to_rocq item (indent + 4)
+        ]
+      ) (List.rev builder.(Builder.constraints))
+    );
+}.
